coq/ZF/Meta/Term/Decl.v
@@ -2,21 +2,21 @@ Require Import Coq.Lists.List.
 
 Require Import ZF.Meta.Ctx.
 Require Import ZF.Meta.Signature.
-Require Import ZF.Meta.Term.
+Require Import ZF.Meta.Term.Syntax.
 Require Import ZF.Meta.Ty.
 
 Import ListNotations.
 
 (* A term declaration records parameters, result sort and optional body.        *)
-Record DeclTerm : Type := mkDeclTerm {
-  para : list Ty;
-  res  : Ty;
-  body : option Term
-}.
+Record Decl : Type := mkDecl
+  { para : list Ty
+  ; res  : Ty
+  ; body : option Term
+  }.
 
 (* The signature of a term declaration seen by identifier application.          *)
-Definition signature (d:DeclTerm) : Signature :=
+Definition signature (d:Decl) : Signature :=
   (para d, res d).
 
 (* A term declaration body is checked in de Bruijn context order.               *)
-Definition ctx (d:DeclTerm) : Ctx := rev (para d).
+Definition ctx (d:Decl) : Ctx := rev (para d).
