coq/ZF/Meta/Test/Class/Equiv.v
@@ -2,9 +2,9 @@ Require Import Coq.Lists.List.
 Require Import Coq.Strings.String.
 
 Require Import ZF.Meta.Ctx.
-Require Import ZF.Meta.HasTy.
+Require Import ZF.Meta.Term.HasTy.
 Require Import ZF.Meta.HasTyIn.
-Require Import ZF.Meta.Term.
+Require Import ZF.Meta.Term.Syntax.
 Require Import ZF.Meta.Ty.
 
 Require Import ZF.Meta.Test.Decl.Class.Equiv.
