coq/ZF/Meta/Test/Set/Pair.v
@@ -3,9 +3,9 @@ Require Import Coq.Strings.String.
 
 Require Import ZF.Meta.Ctx.
 Require Import ZF.Meta.Env.
-Require Import ZF.Meta.HasTy.
+Require Import ZF.Meta.Term.HasTy.
 Require Import ZF.Meta.HasTyIn.
-Require Import ZF.Meta.Term.
+Require Import ZF.Meta.Term.Syntax.
 Require Import ZF.Meta.Ty.
 
 Require Import ZF.Meta.Test.Decl.Class.Equiv.
